feat(library/data/list, library/data/array): theorems needed for new hash_map
Note that hash_map is moved to library_dev, where the more advanced theorems on lists are available

library/init/data/array/basic.lean
@@ -1,7 +1,7 @@
 /-
 Copyright (c) 2017 Microsoft Corporation. All rights reserved.
 Released under Apache 2.0 license as described in the file LICENSE.
-Authors: Leonardo de Moura
+Authors: Leonardo de Moura, Mario Carneiro
 -/
 prelude
 import init.data.nat
@@ -16,14 +16,14 @@ def mk_array {α} (n) (v : α) : array α n :=
 namespace array
 variables {α : Type u} {β : Type w} {n : nat}
 
+def nil {α} : array α 0 :=
+{data := λ ⟨x, h⟩, absurd h (nat.not_lt_zero x)}
+
 def read (a : array α n) (i : fin n) : α :=
 a.data i
 
 def read' [inhabited α] (a : array α n) (i : nat) : α :=
 if h : i < n then a.read ⟨i,h⟩ else default α
-
-lemma read_eq_read' [inhabited α] (a : array α n) (i : nat) (h : i < n) : read a ⟨i, h⟩ = read' a i :=
-by unfold read'; rw [dif_pos h]
 
 def write (a : array α n) (i : fin n) (v : α) : array α n :=
 {data := λ j, if i = j then v else a.read j}
@@ -31,82 +31,92 @@ def write (a : array α n) (i : fin n) (v : α) : array α n :=
 def write' (a : array α n) (i : nat) (v : α) : array α n :=
 if h : i < n then a.write ⟨i, h⟩ v else a
 
-lemma write_eq_write' (a : array α n) (i : nat) (h : i < n) (v : α) : write a ⟨i, h⟩ v = write' a i v :=
-by unfold write'; rw [dif_pos h]
-
-lemma push_back_idx {j n} : j < n + 1 → j ≠ n → j < n :=
-λ h₁ h₂, nat.lt_of_le_and_ne (nat.le_of_lt_succ h₁) h₂
+lemma push_back_idx {j n} (h₁ : j < n + 1) (h₂ : j ≠ n) : j < n :=
+nat.lt_of_le_and_ne (nat.le_of_lt_succ h₁) h₂
 
 def push_back (a : array α n) (v : α) : array α (n+1) :=
 {data := λ ⟨j, h₁⟩, if h₂ : j = n then v else a.read ⟨j, push_back_idx h₁ h₂⟩}
 
-lemma pop_back_idx {j n} : j < n → j < n + 1 :=
-λ h, nat.lt.step h
+lemma pop_back_idx {j n} (h : j < n) : j < n + 1 :=
+nat.lt.step h
 
 def pop_back (a : array α (n+1)) : array α n :=
 {data := λ ⟨j, h⟩, a.read ⟨j, pop_back_idx h⟩}
 
-lemma lt_aux_1 {a b c : nat} : a + c < b → a < b :=
-λ h, lt_of_le_of_lt (nat.le_add_right a c) h
+lemma lt_aux_1 {a b c : nat} (h : a + c < b) : a < b :=
+lt_of_le_of_lt (nat.le_add_right a c) h
 
-lemma lt_aux_2 {n} : n > 0 → n - 1 < n :=
-assume h,
-  have h₁ : 1 > 0, from dec_trivial,
+lemma lt_aux_2 {n} (h : n > 0) : n - 1 < n :=
+have h₁ : 1 > 0, from dec_trivial,
 nat.sub_lt h h₁
 
-lemma lt_aux_3 {n i} : i + 1 < n → n - 2 - i < n  :=
-assume h,
+lemma lt_aux_3 {n i} (h : i + 1 < n) : n - 2 - i < n  :=
 have n > 0,     from lt.trans (nat.zero_lt_succ i) h,
 have n - 2 < n, from nat.sub_lt this (dec_trivial),
 lt_of_le_of_lt (nat.sub_le _ _) this
 
-def foreach_aux (f : fin n → α → α) : Π (i : nat), i < n → array α n → array α n
-| 0     h a :=
-  let i : fin n := ⟨n - 1, lt_aux_2 h⟩ in
-  a.write i (f i (a.read i))
+@[elab_as_eliminator]
+theorem write_ind (a : array α n) (i : fin n) (v : α) (C : fin n → α → Sort w)
+  (Hi : C i v) (Hj : ∀j, i ≠ j → C j (a.read j)) (j) : C j ((a.write i v).read j) :=
+show C j (if i = j then v else read a j), from
+if h : i = j then by rwa [if_pos h, -h]
+else by rw [if_neg h]; exact Hj j h
+
+def foreach_aux (f : fin n → α → α) : Π (i : nat), i ≤ n → array α n → array α n
+| 0     h a := a
 | (j+1) h a :=
-  let i : fin n := ⟨n - 2 - j, lt_aux_3 h⟩ in
-  foreach_aux j (lt_aux_1 h) (a.write i (f i (a.read i)))
+  let i : fin n := ⟨n - 1 - j, nat.sub_one_sub_lt h⟩ in
+  foreach_aux j (le_of_lt h) (a.write i (f i (a.read i)))
 
-def foreach : Π {n}, array α n → (fin n → α → α) → array α n
-| 0     a f:= a
-| (n+1) a f := foreach_aux f n  (nat.lt_succ_self _) a
+def foreach (a : array α n) (f : fin n → α → α) : array α n :=
+foreach_aux f n (le_refl _) a
 
-def map {α} {n} (f : α → α) (a : array α n) : array α n :=
+def map (f : α → α) (a : array α n) : array α n :=
 foreach a (λ _, f)
 
-def map₂ {α} {n} (f : α → α → α) (a b : array α n) : array α n :=
+def map₂ (f : α → α → α) (a b : array α n) : array α n :=
 foreach b (λ i, f (a.read i))
 
-def iterate_aux (f : fin n → α → β → β) : Π (i : nat), i < n → array α n → β → β
-| 0     h a b :=
-  let i : fin n := ⟨n - 1, lt_aux_2 h⟩ in
-  f i (a.read i) b
-| (j+1) h a b :=
-  let i : fin n := ⟨n - 2 - j, lt_aux_3 h⟩ in
-  iterate_aux j (lt_aux_1 h) a (f i (a.read i) b)
+def iterate_aux (a : array α n) (f : fin n → α → β → β) : Π (i : nat), i ≤ n → β → β
+| 0     h b := b
+| (j+1) h b :=
+  let i : fin n := ⟨j, h⟩ in
+  f i (a.read i) (iterate_aux j (le_of_lt h) b)
 
-def iterate : Π {n}, array α n → β → (fin n → α → β → β) → β
-| 0     a b fn := b
-| (n+1) a b fn := iterate_aux fn n (nat.lt_succ_self _) a b
+def iterate (a : array α n) (b : β) (fn : fin n → α → β → β) : β :=
+iterate_aux a fn n (le_refl _) b
 
-def foldl {n} (a : array α n) (b : β) (f : α → β → β) : β :=
+def foldl (a : array α n) (b : β) (f : α → β → β) : β :=
 iterate a b (λ _, f)
 
-def rev_iterate_aux (f : fin n → α → β → β) : Π (i : nat), i < n → array α n → β → β
-| 0 h a b :=
-  let z : fin n := ⟨0, h⟩ in
-  f z (a.read z) b
-| (j+1) h a b :=
-  let i : fin n := ⟨j+1, h⟩ in
-  rev_iterate_aux j (lt_aux_1 h) a (f i (a.read i) b)
+def rev_list (a : array α n) : list α :=
+a.foldl [] (λ v l, v :: l)
 
-def rev_iterate : Π {n : nat}, array α n → β → (fin n → α → β → β) → β
-| 0     a b fn := b
-| (n+1) a b fn := rev_iterate_aux fn n (nat.lt_succ_self _) a b
+def foldl_eq_aux (a : array α n) (b : β) (f : α → β → β) :
+  Π (i : nat) (h : i ≤ n), iterate_aux a (λ _, f) i h b = (iterate_aux a (λ _ v l, v :: l) i h []).foldr f b
+| 0     h := rfl
+| (j+1) h := congr_arg (f (read a ⟨j, h⟩)) (foldl_eq_aux j _)
+
+def foldl_eq (a : array α n) (b : β) (f : α → β → β) : a.foldl b f = a.rev_list.foldr f b :=
+foldl_eq_aux a b f _ _
+
+def rev_iterate_aux (a : array α n) (f : fin n → α → β → β) : Π (i : nat), i ≤ n → β → β
+| 0     h b := b
+| (j+1) h b :=
+  let i : fin n := ⟨j, h⟩ in
+  rev_iterate_aux j (le_of_lt h) (f i (a.read i) b)
+
+def rev_iterate (a : array α n) (b : β) (fn : fin n → α → β → β) : β :=
+rev_iterate_aux a fn n (le_refl _) b
 
 def to_list (a : array α n) : list α :=
 a.rev_iterate [] (λ _ v l, v :: l)
+
+protected def mem (v : α) (a : array α n) : Prop := ∃i, read a i = v
+
+instance : has_mem α (array α n) := ⟨array.mem⟩
+
+theorem read_mem (a : array α n) (i) : read a i ∈ a := exists.intro i rfl
 
 instance [has_to_string α] : has_to_string (array α n) :=
 ⟨to_string ∘ to_list⟩
@@ -118,3 +128,6 @@ meta instance [has_to_tactic_format α] : has_to_tactic_format (array α n) :=
 ⟨tactic.pp ∘ to_list⟩
 
 end array
+
+def list.to_array {α} (l : list α) : array α l.length :=
+{data := λ v, l.nth_le v.1 v.2}
