library/init/data/list/basic.lean
@@ -94,6 +94,11 @@ def remove_all [decidable_eq α] : list α → list α → list α
 | (x :: xs) ys := (if x ∈ ys then remove_all xs ys else x :: remove_all xs ys)
 | [] ys := []
 
+def nth_le : Π (l : list α) (n), n < l^.length → α
+| []       n     h := absurd h (not_lt_zero n)
+| (a :: l) 0     h := a
+| (a :: l) (n+1) h := nth_le l n (le_of_succ_le_succ h)
+
 def head [inhabited α] : list α → α
 | []       := default α
 | (a :: l) := a
@@ -132,6 +137,11 @@ def filter (p : α → Prop) [decidable_pred p] : list α → list α
 def find [decidable_eq α] : α → list α → nat
 | a []       := 0
 | a (b :: l) := if a = b then 0 else succ (find a l)
+
+def drop : ℕ → list α → list α
+| 0 r := tail r
+| (succ n) [] := []
+| (succ n) (x::r) := x :: drop n r
 
 def dropn : ℕ → list α → list α
 | 0 a := a
