library/init/data/option/instances.lean
@@ -28,3 +28,9 @@ instance : alternative option :=
 { option.monad with
   failure := @none,
   orelse  := @option_orelse }
+
+lemma option.eq_of_eq_some {α : Type u} : Π {x y : option α}, (∀z, x = some z ↔ y = some z) → x = y
+| none     none     h := rfl
+| none     (some z) h := option.no_confusion ((h z).2 rfl)
+| (some z) none     h := option.no_confusion ((h z).1 rfl)
+| (some z) (some w) h := option.no_confusion ((h w).2 rfl) (congr_arg some)
